src/typechecker/FStar.TypeChecker.Rel.fsti
@@ -49,6 +49,7 @@ val solve_deferred_constraints: env -> guard_t -> guard_t
 val solve_non_tactic_deferred_constraints: maybe_defer_flex_flex:bool -> env -> guard_t -> guard_t
 val discharge_guard_no_smt    : env -> guard_t -> guard_t
 val discharge_guard           : env -> guard_t -> guard_t
+val query_formula             : env -> formula -> list FStar.Errors.error
 val force_trivial_guard       : env -> guard_t -> unit
 val resolve_implicits         : env -> guard_t -> guard_t
 val resolve_implicits_tac     : env -> guard_t -> guard_t
